src/Init/Data/Nat/Basic.lean
@@ -47,6 +47,7 @@ def blt (a b : Nat) : Bool :=
 @[simp] theorem zero_eq : Nat.zero = 0 := rfl
 @[simp] theorem add_eq : Nat.add x y = x + y := rfl
 @[simp] theorem mul_eq : Nat.mul x y = x * y := rfl
+@[simp] theorem sub_eq : Nat.sub x y = x - y := rfl
 @[simp] theorem lt_eq : Nat.lt x y = (x < y) := rfl
 @[simp] theorem le_eq : Nat.le x y = (x ≤ y) := rfl
 
